reset tr/Abstract_tree.thy to commit 299aef8714bff7dfe2dafb081d90033f772bcecc

src/isabelle/tr/Abstract_tree.thy
@@ -80,9 +80,6 @@ record ('k,'v) leaf_frame =
 
 datatype ('r,'k,'v) frame = Frm_I "('r,'k) node_frame" | Frm_L "('k,'v) leaf_frame"
 
-definition frm_to_values_number :: "('r,'k,'v) frame \<Rightarrow> nat" where
-  "frm_to_values_number frm = (case frm of Frm_I nf \<Rightarrow> (nf |> nf_n) + 1 | Frm_L lf \<Rightarrow> lf |> lf_kvs |> length)"
-
 definition key_to_v :: "('k,'v) leaf_frame => 'k key => 'v value_t option" where
   "key_to_v lf k == (lf |> lf_kvs |> map_of) k"
 
@@ -149,24 +146,7 @@ fun page_ref_to_tree :: "('bs,'k,'r,'v) ctxt_p2f_t =>  ('r,'bs) store => 'r page
           let ks = (nf|>nf_ks) in
           let rs = (nf|>nf_rs) :: (nat => 'r page_ref) in
           let f0 = (% r. page_ref_to_tree c0 s0 r n') :: ('r page_ref => ('k,'v) tree option) in
-          let prop =
-           let not_empty_frames =
-            let not_empty = (% r.
-              (case page_ref_to_frame c0 s0 r of
-              None => False  (* attempt to access missing page *)
-              | Some frm => (
-                case frm of 
-                  Frm_I(nf) => (nf|>nf_n) \<noteq> 0 (* this is not necessary *)
-                  | Frm_L(lf) => \<not> (lf|>lf_kvs|>List.null))))
-            in
-            n \<noteq> 0
-            \<and>
-            (! (m::nat). m <= n --> m |> rs |> not_empty)
-          in
-            not_empty_frames
-            \<and>
-            (! (m::nat). m <= n --> m |> rs |> f0 |> is_Some)
-          in
+          let prop = (! (m::nat). m <= n --> m |> rs |> f0 |> is_Some) in (* we use \<le> because the number of subtrees to create is n (number of keys) + 1 --since we start from index 0, it is just n*)
           case prop of
           True => (Some(Tr_nd(n,ks,(% (m::nat). m |> rs |> f0 |> dest_Some))))
           | False => (Error |> rresult_to_option))  (* Frm_I was not wellformed - prop was false *)
@@ -200,12 +180,10 @@ section "(given node_frame) key_to_ref, ctxt_k2r_t"
 
 
 (* NB we need some properties of these functions for correctness 
-
 This abstracts from the particular find implementation. Essentially, at a non-leaf node, we need to map
 a key to a page ref, from which we can continue the find. The property this function should have is
 that, given a key, if there is a value corresponding to the key (which is unique), then the 
 returned page ref identifies the relevant subtree.
-
 *)
 datatype ('bs,'k,'r,'v) key_to_ref = Key_to_ref "('r,'k) node_frame => 'k key => 'r page_ref" 
 (* datatype ('bs,'k,'r,'v) key_to_v = Key_to_v "('k,'v) leaf_frame => 'k key => 'v option"  (* may be no such v *) - there is only one impl! *)
@@ -246,7 +224,7 @@ definition find_state_to_page_ref :: "('bs,'k,'r,'v) find_state => 'r page_ref" 
 
 definition fs_step :: "('bs,'k,'r,'v) ctxt_k2r_t
   => (('r,'bs) store * ('bs,'k,'r,'v) find_state) 
-  => (('r,'bs) store * ('bs,'k,'r,'v) find_state) option" where
+  => (('bs,'k,'r,'v) find_state) option" where
   "fs_step ctxt1 s0fs0 == (
   let (s0,fs0) = s0fs0 in
   case fs0 of
@@ -260,11 +238,11 @@ definition fs_step :: "('bs,'k,'r,'v) ctxt_k2r_t
       Frm_I nf => (
         let k2r = ((ctxt1|>key_to_ref)|>dest_key_to_ref) in
         let r' = k2r nf k0 in
-        Some(s0, Fs_l (fsl (| fsl_r := r' |))))
+        Some(Fs_l (fsl (| fsl_r := r' |))))
       | Frm_L lf => (
         let k2v = key_to_v in
         let v = k2v lf k0 in
-        Some(s0, Fs_r (| fsr_r = r0, fsr_v = v |)))))
+        Some(Fs_r (| fsr_r = r0, fsr_v = v |)))))
   | Fs_r fsr => (Error |> rresult_to_option))"  (* attempt to step Fs_r *)
 
 
@@ -276,52 +254,72 @@ text "iterate the fs_step function n times"
 definition fs_step_as_fun :: "('bs,'k,'r,'v) ctxt_k2r_t 
   => tree_height
   => (('r,'bs) store * ('bs,'k,'r,'v) find_state) 
-  => (('r,'bs) store * ('bs,'k,'r,'v) find_state)" where
+  => (('bs,'k,'r,'v) find_state)" where
   "fs_step_as_fun ctxt1 n0 s0fs0 == (
-  let f0 = % x. x |> (fs_step ctxt1) |> dest_Some in
-  (f0^^n0) s0fs0)"
+  let (s0,fs0) = s0fs0 in
+  let f0 = % x. (s0,x) |> (fs_step ctxt1) |> dest_Some in
+  (Nat.funpow n0 f0) fs0)"
 
 
 section "wellformedness predicates"
 
-definition wf_ctxts where 
-  "wf_ctxts ctxt_k2r s0 r0 n0 == (
-     let ctxt_p2f = ctxt_p2f_t.truncate ctxt_k2r in
-     case n0 of
-      0 \<Rightarrow>
-      (case page_ref_to_frame ctxt_p2f s0 r0 of
-      Some (Frm_L(_)) \<Rightarrow> True
-      | _ \<Rightarrow> False)
-     | Suc n' \<Rightarrow> (
-     case page_ref_to_frame ctxt_p2f s0 r0 of
-       Some (Frm_I(nf)) \<Rightarrow>
-         let n = (nf|>nf_n) in
-         let ks = (nf|>nf_ks) in
-         let rs = (nf|>nf_rs) :: (nat => 'r page_ref) in
-         let k2r :: (('r,'k) node_frame => 'k key => 'r page_ref)= (ctxt_k2r |> key_to_ref |> dest_key_to_ref) in
-          (\<exists> m' \<le> n . ! k .
-          let key_p_ref = m'|>rs in
-          (* the page_ref returned must be among the inodes page_refs *)
-          (k2r nf k) = key_p_ref
-          \<and>
-          (* the key can be only in the subtree generated by the m' page_ref *)
-          (
-            (page_ref_key_to_v ctxt_p2f s0 r0 (Suc n') k = page_ref_key_to_v ctxt_p2f s0 key_p_ref (n') k)
-            \<and>
-            (! m. m \<le> n \<and> m \<noteq> m' \<longrightarrow> (page_ref_key_to_v ctxt_p2f s0 r0 (Suc n') k \<noteq> page_ref_key_to_v ctxt_p2f s0 (m|>rs) (n') k))
-          )
-          ) 
-     | _ \<Rightarrow> False))"
+(* FIXME obviously the following need to be filled in properly *)
 
-fun wf_store:: "('bs,'k,'r,'v) ctxt_k2r_t => ('r,'bs) store => 'r page_ref => tree_height => bool" where
-  "wf_store ctxt_k2r s0 r0 0 = is_Some (page_ref_to_tree (ctxt_p2f_t.truncate ctxt_k2r) s0 r0 0)"
-  | "wf_store ctxt_k2r s0 r0 (Suc n') = (
-      is_Some (page_ref_to_tree (ctxt_p2f_t.truncate ctxt_k2r) s0 r0 (Suc n'))
-      &
-      wf_ctxts ctxt_k2r s0 r0 (Suc n')
+definition wf_ctxt:: "('bs,'k,'r,'v) ctxt_k2r_t => bool" where
+  "wf_ctxt ctxt == True"
 
-& True)
-  "
+definition wf_ctxt1:: "('bs,'k,'r,'v) ctxt_k2r_t => bool" where
+  "wf_ctxt1 ctxt1 == 
+  ! s0 r0 ctxt nf k0 r' v0 n0 m1 m1'.
+(ctxt_p2f_t.truncate ctxt1 = ctxt)
+(* if r0 is not a leaf *)
+& (page_ref_to_frame ctxt s0 r0 = Some (Frm_I nf))
+(* and the map exists at r0 *)
+& (page_ref_to_map ctxt s0 r0 n0 = Some m1)
+(* and we descend to r' *)
+& (dest_key_to_ref (key_to_ref ctxt1) nf k0 = r')
+(* and the map exists at r' *)
+& (page_ref_to_map ctxt s0 r' (n0 - Suc 0) = Some m1')
+(* then the maps agree, at least for the key *)
+& (m1 k0 = v0)
+--> (m1' k0 = v0)
+"
+
+
+(*
+definition wf_store_page_ref_to_map_none :: "('bs,'k,'r,'v) ctxt_k2r_t => ('r,'bs) store => tree_height => 'r page_ref => bool" where
+  "wf_store_page_ref_to_map_none  c1 s0 n0 r0 == (
+    let c0 = ctxt_p2f_t.truncate c1 in
+    ((page_ref_to_map c0 s0 r0 n0 = None) --> False)
+  )"
+*)
+
+definition wf_store_page_ref_to_map :: "('bs,'k,'r,'v) ctxt_k2r_t => ('r,'bs) store => tree_height => 'r page_ref => bool" where
+  "wf_store_page_ref_to_map  c1 s0 n0 r0 == (
+    let c0 = ctxt_p2f_t.truncate c1 in
+(! m1 r' nf k0 . ((
+(* if we have a map at r0 *)
+(page_ref_to_map c0 s0 r0 n0 = Some m1)
+& (page_ref_to_frame c0 s0 r0 = Some (Frm_I nf))
+(* and we follow the key to r' *)
+& (dest_key_to_ref (c1|>key_to_ref) nf k0 = r')
+(* then we still have a map *)
+& (page_ref_to_map c0 s0 r' (n0 - Suc 0) = None)
+) --> False
+))  (* FIXME does this follow from page_ref_to_map ~= None? FIXME isn't this a basic property of the defn of page_ref_to_map/page_ref_to_tree? *)
+& (page_ref_to_map c0 s0 r0 n0 ~= None)    
+  )"
+
+
+definition wf_store:: "('bs,'k,'r,'v) ctxt_k2r_t => ('r,'bs) store => tree_height => 'r page_ref => bool" where
+  "wf_store c1 s0 n0 r0 == (
+(*    wf_store_page_ref_to_map_none c1 s0 n0 r0 *)
+    wf_store_page_ref_to_map c1 s0 n0 r0
+& True)"
+
+(*
+  
+*)
 
 section "correctness of fs_step"
 
@@ -342,279 +340,246 @@ definition fs_step_invariant :: "('bs,'k,'r,'v) ctxt_p2f_t
       let v' = (fsr|>fsr_v) in
       v' = v0))"
 
+(* FIXME in the following we want to eliminate n0 and v0 explicit arguments, and phrase as a
+simple invariant; v0 can be a parameter of the invariant; how do we get n0? just say I v0 == ! n0. wf_store s0 n0... --> *)
 lemma fs_step_is_invariant: "
-  ! (ctxt1::('bs,'k,'r,'v) ctxt_k2r_t) s0 fs0 n0 v0.
+  ! (ctxt1::('bs,'k,'r,'v) ctxt_k2r_t) ctxt s0 fs0 n0 v0.
   ((ctxt_p2f_t.truncate ctxt1) = ctxt)
-  --> (case fs0 of Fs_l fsl \<Rightarrow> fsl |> fsl_r | Fs_r fsr \<Rightarrow> fsr |> fsr_r ) = r0
-  --> wf_store ctxt1 s0 r0 n0 
+  --> wf_ctxt1 ctxt1 & wf_store ctxt1 s0 n0 (fs0|>find_state_to_page_ref)
   --> (
   fs_step_invariant ctxt (s0,fs0) n0 v0 --> (
   let x = fs_step ctxt1 (s0,fs0) in
   case x of 
   None => True  (* if we are at a Fs_r, no further facts are available *)
-  | Some (s',fs') => (
+  | Some (fs') => (
     (* n0 could be 0? but then fs' is Fs_r? *)
-    fs_step_invariant ctxt (s',fs') (n0 - 1) v0)))"
-
-apply (simp add:Let_def)
-apply rule+
-apply (case_tac n0)
- (* 0 *)
- apply (simp add:is_Some_def)
- apply (erule exE)
- apply (rename_tac frm)
- apply (simp add:fs_step_invariant_def)
- apply (case_tac "fs0")
-  apply (rename_tac fsl)
-  (* fs0 = Fs_l fsl*)
-  apply simp
-  apply (thin_tac "fs0 = ?x")
-  apply (simp add:fs_step_def)
-  apply (subgoal_tac "? k0. (fsl |> fsl_k) = k0") prefer 2 apply force
-  apply (erule exE)+
-  apply simp
-  apply (subgoal_tac "? m_frm'. page_ref_to_frame ctxt s0 r0 = m_frm'") prefer 2 apply force
-  apply (erule exE)
-  apply simp
-  apply (case_tac "m_frm'")
-   (* m_frm' = None *)
-   apply simp
-   
-   apply (rename_tac frm')
-   (* m_frm' = Some frm' *)
-   apply simp
-   apply (thin_tac "m_frm' = Some frm'")
-   apply (case_tac "frm'")
-    (* frm' = Frm_I _ *)
-    apply (simp add:rev_apply_def rresult_to_option_def)
-
-    (* frm' = Frm_L _ *)
-    apply (simp add:rev_apply_def rresult_to_option_def fs_step_invariant_def page_ref_key_to_v_def 
-      page_ref_to_map_def page_ref_to_kvs_def kvs_to_map_def key_to_v_def)
-
-  (* fs0 = Fs_l fsl*)
-  apply (simp add:fs_step_def)
-
- (* n0 = Suc n' *)
- apply (simp add:is_Some_def)
- apply (erule conjE)+
- apply (erule exE)
- apply (rename_tac "tree")
- apply (subgoal_tac "? m_frm. page_ref_to_frame ctxt s0 (case fs0 of Fs_l fsl \<Rightarrow> fsl |> fsl_r | Fs_r fsr \<Rightarrow> fsr |> fsr_r) = m_frm") prefer 2 apply force
- apply (erule exE)
- apply simp
- apply (case_tac "m_frm")
-  (* m_frm = None *)
-  apply simp
-
-  apply (rename_tac frm)
-  (* m_frm = Some frm *)
-  apply simp
-  apply (case_tac fs0)
+    fs_step_invariant ctxt (s0,fs') (n0 - 1) v0)))"
+  apply(rule)+
+  apply(elim conjE)
+  apply(subgoal_tac "? x. fs_step ctxt1 (s0, fs0) = x")
    prefer 2
-   (* fs0 = Fs_r find_state_r_ext *)
-   apply (simp add:fs_step_def)
+   apply(force)
+  apply(erule exE)
+  apply(simp add: Let_def)
+  apply(case_tac x)
+   (* none *)
+   apply(force)
 
-   apply (rename_tac fsl)
-   (* fs0 = Fs_l fsl*)
-   apply (case_tac "frm") 
+   (* x = Some a *)
+   apply(simp)
+   apply(rename_tac "fs'")
+   apply(simp add: fs_step_def)
+   apply(case_tac fs0)
     prefer 2
-    (* frm = Frm_L _*)
-    apply simp
+    apply(force)
+   (* fs0 = Fs_l find_state_l_ex *)
+   apply(simp)
+   apply(rename_tac "fsl")
+   apply(subgoal_tac "? r0. (fsl|>fsl_r) = r0")
+    prefer 2 apply(force)
+   apply(subgoal_tac "? k0. (fsl|>fsl_k) = k0 ")
+    prefer 2 apply(force)
+   apply(erule exE)+
+   apply(case_tac " (page_ref_to_frame (ctxt_p2f_t.truncate ctxt1) s0 r0)")
+    apply(force)
 
-    apply (rename_tac nf)
-    (* frm = Frm_I nf*)    
-    apply (simp add:Let_def wf_ctxts_def)
-    apply (erule exE)+
-    apply (case_tac " 0 < nf |> nf_n \<and>
-             (\<forall>m\<le>nf |> nf_n.
-                 m |> (nf |> nf_rs) |>
-                 (\<lambda>r. case page_ref_to_frame ctxt s0 r of None \<Rightarrow> False | Some (Frm_I nf) \<Rightarrow> nf |> nf_n \<noteq> 0 | Some (Frm_L lf) \<Rightarrow> \<not> lf |> lf_kvs |> List.null)) \<and>
-             (\<forall>m\<le>nf |> nf_n. m |> (nf |> nf_rs) |> (\<lambda>r. page_ref_to_tree ctxt s0 r nat) |> is_Some)")
-    prefer 2
-     (* prop = false *)
-     apply simp
+    (*  (page_ref_to_frame (ctxt_p2f_t.truncate ctxt1) s0 r0) = Some r' *)
+    apply(rename_tac frm')
+    apply(simp)
+    apply(case_tac frm')
+     (**********)
+     (* frm' = Frm_I node_frame_ext *)
+     apply(rename_tac nf)  (* nf = node_frame *)
+     apply(simp)
+     apply(thin_tac "fs0 = ?x")
+     apply(thin_tac "frm' = ?x")
+     apply(thin_tac "x=?x")
+     apply(subgoal_tac "? fsl'. (fsl\<lparr>fsl_r := (ctxt1 |> key_to_ref |> dest_key_to_ref) nf k0\<rparr>) = fsl'")
+      prefer 2 apply(force)
+     apply(erule exE)
+     apply(simp)
+     apply(subgoal_tac "? r'. (ctxt1 |> key_to_ref |> dest_key_to_ref) nf k0 = r'")
+      prefer 2 apply(force)
+     apply(erule exE)
+     (* note how this goal is concise and readable *)
+     apply(simp add: fs_step_invariant_def)
+     apply(drule_tac t="fs'" in sym)
+     apply(simp)
+     apply(thin_tac "fs' = ?x")
+     apply(drule_tac t="fsl'" in sym)
+     apply(simp)
+     apply(subgoal_tac "fsl\<lparr>fsl_r := r'\<rparr> = (| fsl_k = k0, fsl_r = r' |)") prefer 2 apply (metis (full_types) find_state_l.surjective find_state_l.update_convs(2) old.unit.exhaust rev_apply_def) 
+     apply(thin_tac "fsl' = fsl\<lparr>fsl_r := r'\<rparr> ")
+     apply(simp)
+     apply(simp add: rev_apply_def)
+     apply(simp add: page_ref_key_to_v_def)
+     (* page_ref_to_map could be none or some *)
+     apply(subgoal_tac "? m0. (page_ref_to_map (ctxt_p2f_t.truncate ctxt1) s0 r0 n0) = m0")
+      prefer 2 apply(force)
+     apply(erule exE)
+     apply(simp)
+     apply(case_tac m0)
+      (* m0 = None *)
+      apply(simp)
+      (* this case ruled out by wellformedness - page_ref_to_map cannot be None *)
+      apply (metis find_state.simps(5) find_state_to_page_ref_def rev_apply_def wf_store_def wf_store_page_ref_to_map_def)
+      
+      (* m0 = Some a *)
+      apply(rename_tac m1)
+      apply(simp)
+      apply(thin_tac "m0 = ?x")
+      apply(subgoal_tac "? m0'.  (page_ref_to_map (ctxt_p2f_t.truncate ctxt1) s0 r' (n0 - Suc 0)) = m0'")
+       prefer 2 apply(force)
+      apply(erule exE)
+      apply(simp)
+      apply(case_tac "m0'")
+       (* none - ruled out because m0 is_Some --> m0' is_Some ; FIXME sledgehammer should get this *)
+       apply(simp)
+       apply(simp add: wf_store_def wf_store_page_ref_to_map_def Let_def)
+       apply(elim conjE)
+       apply(erule exE)
+       apply(simp add: page_ref_to_map_def page_ref_to_kvs_def rev_apply_def find_state_to_page_ref_def)
+       apply(elim exE conjE)
+       apply(simp)
+       apply (metis option.distinct(1))  
 
-     (* prop = true *)
-     apply simp
-     apply (erule conjE)+
-     apply (drule_tac x="fsl|>fsl_k" in spec)
-     apply (erule conjE)+
-     apply (simp add:fs_step_def)
-     apply (simp add:fs_step_invariant_def)
-     apply (drule_tac t="v0" in sym)
-     apply (simp add: rev_apply_def)
-done
-
-section "frame_to_page, ctxt_f2p"
-
-(* encoding of pages *)
-datatype ('bs,'k,'r,'v) frame_to_page = F2p "('r,'k,'v) frame \<Rightarrow> 'bs page"
-
-definition dest_f2p :: "('bs,'k,'r,'v) frame_to_page => ('r,'k,'v) frame \<Rightarrow> 'bs page" where
-  "dest_f2p x = (case x of F2p f => f)"
-
-record ('bs,'k,'r,'v) ctxt_f2p_t = "('bs,'k,'r,'v) ctxt_k2r_t" +
-  ctxt_f2p :: "('bs,'k,'r,'v) frame_to_page"
-  
-section "insert, insert_state, insert_step"
-
-type_synonym 'r root_p_ref = "'r page_ref"
-
-record ('bs,'k,'r,'v) ctxt_insert_t = "('bs,'k,'r,'v) ctxt_f2p_t" +
-  maxNumValues  :: nat
-  free_page_ref :: "('r,'bs) store \<Rightarrow> ('r page_ref * ('r,'bs) store)" (* need to constraint this so that the returned page_ref is not in the store *)
-  (* I need an interface that alters Fr_I *)
-  new_nf :: "('r,'k) node_frame"
-  (*add_key_nf should update the nf_n field of the node_frame when key is Some *)
-  add_key_page_ref_nf :: "('k key) option \<Rightarrow> 'r page_ref \<Rightarrow> ('r,'k) node_frame \<Rightarrow> ('r,'k) node_frame"
-  (* [sust_page_ref_nf old new frm] substitute a given page_ref with another, if the first one is present *)
-  subst_page_ref_nf :: "'r page_ref \<Rightarrow> 'r page_ref \<Rightarrow> ('r,'k) node_frame \<Rightarrow> ('r,'k) node_frame"
-
-fun ins :: "('k * 'v) \<Rightarrow> ('k * 'v) list \<Rightarrow> ('k * 'v) list" where
-  "ins kv [] = [kv]"
-  | "ins kv (kv'#kvs) =
-    (if (fst kv) = (fst kv')
-    (* update entry *)
-    then kv#kvs
-    else kv'#(ins kv kvs))
-  "
-
-(* insert *)
-record ('k,'r,'v) insert_state_t =
-  ist_kv :: "('k key * 'v value_t)"
-  ist_r  :: "'r page_ref"
-
-datatype ('k,'r,'v) insert_state =
-    Ist_root "('k,'r,'v) insert_state_t" (* case in which root is full and we create a new root *)
-  | Ist_insert_nonfull "('k,'r,'v) insert_state_t"
-  | Ist_done
-
-definition split_child :: "('bs,'k,'r,'v) ctxt_insert_t
-  => (('r,'bs) store * ('r page_ref * ('r,'k) node_frame) * ('r page_ref * ('r,'k,'v) frame)) 
-  => (('r,'bs) store * ('r,'k) node_frame)" where
-(* NB: having a node_frame in the result allows us to spare a READ to disk (although likely that data would be in the cache) *)
-  "split_child ctxt c0 = (
-  let (s0, (x_r,x_nf),(y_r,y_frm)) = c0 in
-  (* we need to allocate 2 new nodes *)
-  let (z_r,s0) = (ctxt |> free_page_ref) s0 in
-  let (y_r',s0) = (ctxt |> free_page_ref) s0 in
-  (* we substitute y_r with y_r' in x_nf*)
-  let x_nf = (ctxt |> subst_page_ref_nf) y_r y_r' x_nf in    
-  let f2p = ((ctxt_f2p_t.truncate ctxt) |> ctxt_f2p |> dest_f2p) in
-  let add_kpr_nf = (ctxt |> add_key_page_ref_nf) in
-  let ((x_r,x_nf'),(y_r',y_frm'),(z_r,z_frm)) = 
-    (case y_frm of
-    Frm_L y_lf \<Rightarrow>
-      let kvs = y_lf |> lf_kvs in
-      (* second half of the entries *)
-      let kvs_2 = (drop ((length kvs) div 2) kvs) in
-      (* first half of the entries *)
-      let kvs_1 = (take ((length kvs) div 2) kvs) in
-      (* FIXME likely I need to insert key and page_ref together in a frame to permit the right positioning of them *)  
-      (* we update the parent node with z
-      and we *copy* the median key (i.e. the first key of the kvs_2) of lf*)
-      (* NB: if we are splitting nodes (in ist_step) they cannot be empty, so hd cannot be undefined *)
-      let x_nf' = add_kpr_nf (Some (fst (hd kvs_2))) z_r x_nf in
-      ((x_r,x_nf'),(y_r',(Frm_L \<lparr> lf_kvs = kvs_1 \<rparr>)),(z_r,(Frm_L \<lparr> lf_kvs = kvs_2 \<rparr>)))
-    | Frm_I y_nf \<Rightarrow>
-      let n  = (y_nf|>nf_n)  in
-      let ks = (y_nf|>nf_ks) in
-      let rs = (y_nf|>nf_rs) :: (nat => 'r page_ref) in
-      let median_key = ks (n div 2) in
-      (* we copy the largest keys and page_refs in the new node z, the median key is excluded though (it is going in the parent )*)
-      let z_nf = add_kpr_nf None (rs ((n div 2)+1)) (ctxt |> new_nf) in
-      let z_nf = foldl (% a n . (add_kpr_nf (Some (ks n)) (rs (n+1)) a) ) z_nf [(n div 2)+1..< n] in
-      (* we delete the largest keys and page_refs from y (i.e. we create a new nf with the smallest keys) *)
-      let y_nf' = add_kpr_nf (None) (rs 0) (ctxt |> new_nf) in
-      let y_nf' = foldl (% a n . (add_kpr_nf (Some (ks n)) (rs (n+1)) a) ) y_nf' [0..<(n div 2)] in
-      (* we update the parent node with z and the median_key *)
-      let x_nf' = add_kpr_nf (Some median_key) z_r x_nf in
-      ((x_r,x_nf'),(y_r',(Frm_I y_nf')),(z_r,(Frm_I z_nf))))
-  in
-  (* we update the store *)
-  (* the new frame contains the second half of the old frame data *)
-  let s1 = Store ((dest_store s0) (z_r \<mapsto> (f2p z_frm))) in
-  (* the old frame contains the first half of the old frame data *)
-  let s2 = Store ((dest_store s1) (y_r' \<mapsto> (f2p y_frm'))) in
-  (* the parent frame got the median key and the new page_refs *)
-  let s3 = Store ((dest_store s2) (x_r \<mapsto> (f2p (Frm_I x_nf')))) in
-  (s3,x_nf'))"
-
-definition ist_step :: "('bs,'k,'r,'v) ctxt_insert_t
-  => (('r,'bs) store * 'r root_p_ref * ('k,'r,'v) insert_state) 
-  => (('r,'bs) store * 'r root_p_ref * ('k,'r,'v) insert_state) option" where
-  "ist_step ctxt s0ist0 = (
-  let (s0,root,ist0) = s0ist0 in
-  let ctxt_f2p_r = (ctxt_f2p_t.truncate ctxt) in
-  let f2p = (ctxt_f2p_r |> ctxt_f2p |> dest_f2p) in
-  let ctxt_k2r_r = ctxt_k2r_t.truncate ctxt_f2p_r in
-  let k2r = ((ctxt_k2r_r|>key_to_ref)|>dest_key_to_ref) in
-  let ctxt_p2f_r = ctxt_p2f_t.truncate ctxt_k2r_r in
-  let add_kpr_nf = (ctxt |> add_key_page_ref_nf) in
-  case ist0 of
-    Ist_root ist \<Rightarrow>
-    let r0 = (ist|>ist_r) in
-    let (k0,v0) = (ist|>ist_kv) in
-    (* new root page_ref to duplicate tree (we want to be able to build the old tree without the new entry after the insert) *)
-    let (r0',s0) = (ctxt |> free_page_ref) s0 in
-    (case (page_ref_to_frame ctxt_p2f_r s0 r0) of 
-    None => (Error |> rresult_to_option)  (* invalid page access *)
-    | Some frm => (
-      case (frm_to_values_number frm = (ctxt |> maxNumValues)) of
-       True \<Rightarrow>
-       (* root is full, we need to create a new root *)
-       let nf_r = (ctxt |> new_nf) in
-       (* the old root node is a child *)
-       let nf_r = add_kpr_nf None r0 nf_r in
-       (* split_child updates the store with the new (page_ref, page)*)
-       let (s1,_) = split_child ctxt (s0,(r0',nf_r),(r0,frm)) in
-       Some (s1,r0',Ist_insert_nonfull(ist\<lparr> ist_r := r0'\<rparr>))
-       | False \<Rightarrow>
-       (* we need to duplicate the root in the store *)
-       let s1 = Store ((dest_store s0) (r0' \<mapsto> (f2p frm))) in
-       Some (s1,r0',Ist_insert_nonfull(ist\<lparr> ist_r := r0'\<rparr>))))
-  | Ist_insert_nonfull ist \<Rightarrow>
-    let r0 = (ist|>ist_r) in
-    let (k0,v0) = (ist|>ist_kv) in
-    (case (page_ref_to_frame ctxt_p2f_r s0 r0) of 
-    None => (Error |> rresult_to_option)  (* invalid page access *)
-    | Some frm => ( 
-      case frm of
-      Frm_L lf \<Rightarrow>
-        (* in a leaf we just update the list of entries with the new one *)
-        let frm' = Frm_L \<lparr> lf_kvs = ins (k0,v0) (lf |> lf_kvs) \<rparr> in
-        (* and we update the store *)
-        let s1 = Store ((dest_store s0) (r0 \<mapsto> (f2p frm'))) in
-        Some (s1,root,Ist_done)
-      | Frm_I nf \<Rightarrow>
-        (* we need to find the child containing k0 *)
-        let r' = k2r nf k0 in
-        (* we resolve the child *)
-        (case (page_ref_to_frame ctxt_p2f_r s0 r0) of
-        None => (Error |> rresult_to_option)  (* invalid page access *)
-        | Some child_frm => (
-          case (frm_to_values_number child_frm = (ctxt |> maxNumValues)) of
-          True \<Rightarrow>
-            (* the child is full: we need to split it *)
-            let (s1,nf') = split_child ctxt (s0,(r0,nf),(r',child_frm)) in
-            (* split changed the parent frame, so we need to look for the child containing k0 again *)
-            let r'' = k2r nf' k0 in
-            Some (s1,root,Ist_insert_nonfull(ist\<lparr> ist_r := r''\<rparr>))
-          | False \<Rightarrow>
-          (** substitute r' with a new page_ref and substitute it with the  r' in the contents of r0*)
-          let (r'',s0) = (ctxt |> free_page_ref) s0 in
-          (* add a clone of the child (with a different page_ref) to the store *)
-          let s1 = Store ((dest_store s0) (r'' \<mapsto> (f2p child_frm))) in
-          (* update r0 contents with r'' instead of r' *)
-          let frm' = (Frm_I ((ctxt |> subst_page_ref_nf) r' r'' nf)) in
-          let s2 = Store ((dest_store s1) (r0 \<mapsto> (f2p frm'))) in
-          Some (s2,root,Ist_insert_nonfull(ist\<lparr> ist_r := r''\<rparr>)))
-       )))
-  | Ist_done \<Rightarrow> (Error |> rresult_to_option))"  (* attempt to step Ist_done *)
+       (* m0' = Some a *)
+       apply(rename_tac "m1'")
+       apply(simp)
+       apply(thin_tac "m0'=?x")
+       (* m1 k0 = v0 --> m1' k0 = v0 ; this holds by wellformedness of key_to_ref, and page_ref_to_map Suc *)
+       apply(simp add: wf_ctxt1_def)
+       apply(force)
 
 
-section "correctness of ist_step"
+     (* frm' = Frm_L leaf_frame_ext - easy case? *)
+     apply(rename_tac lf)
+     apply(simp)
+     apply(thin_tac "fs0 = ?x")
+     apply(thin_tac "frm' = ?x")
+     apply(thin_tac "x=?x")
+     (* we have got to a leaf, and at frm' we return Fs_r *)
+     apply(subgoal_tac "? fsr'.  \<lparr>fsr_r = r0, fsr_v = key_to_v lf k0\<rparr> = fsr'")
+      prefer 2 apply(force)
+     apply(erule exE)
+     apply(simp)
+     apply(subgoal_tac "? v'. key_to_v lf k0 = v'")
+      prefer 2 apply(force)
+     apply(erule exE)
+     apply(simp add: fs_step_invariant_def)
+     apply(drule_tac t="fs'" in sym)
+     apply(simp)
+     apply(thin_tac "fs' = ?x")
+     apply(drule_tac t="fsr'" in sym)
+     apply(simp)
+     apply(thin_tac "fsr' = ?x")
+     apply(simp)
+     apply(simp (no_asm) add: rev_apply_def)
+     apply(simp add: page_ref_key_to_v_def)
+     (* page_ref_to_map could be none or some *)
+     apply(subgoal_tac "? m0. (page_ref_to_map (ctxt_p2f_t.truncate ctxt1) s0 r0 n0) = m0")
+      prefer 2 apply(force)
+     apply(erule exE)
+     apply(simp)
+     apply(case_tac m0)
+      (* m0 = None *)
+      apply(simp)
+      (* the map at r0 is none ; but we have a leaf frame; contradiction; FIXME the following should be simplified *)
+      (*
+      apply(simp add: page_ref_to_frame_def)
+      apply(case_tac "ref_to_page s0 r0") apply(force)
+      apply(simp)
+      apply(rename_tac p0)
+      *)
+      (*  ref_to_page s0 r0 = Some p0 *)
+      apply(simp add: page_ref_to_map_def)
+      apply(case_tac "page_ref_to_kvs (ctxt_p2f_t.truncate ctxt1) s0 r0 n0") 
+       (* page_ref_to_kvs = none *)
+       apply(simp)
+       (* apply(simp add: ref_to_page_def) *)
+       apply(simp add: page_ref_to_kvs_def)
+       apply(simp add: rev_apply_def)
+       apply(case_tac "page_ref_to_tree (ctxt_p2f_t.truncate ctxt1) s0 r0 n0")
+        (* page_ref_to_tree (ctxt_p2f_t.truncate ctxt1) s0 r0 n0 = none *)
+        (* page_ref_to_tree defined by primrec *)
+        apply(case_tac n0)
+         apply(force)
+         (*
+         apply(simp)
+         apply(simp add: page_ref_to_frame_def)
+         apply(force simp add: ref_to_page_def rev_apply_def)
+         *)
 
+         (* n0 = suc nat *)
+         apply(rename_tac n0')
+         apply(simp)
+         apply(simp add: page_ref_to_frame_def)
+         apply(simp add: ref_to_page_def rev_apply_def)
+         apply(case_tac "dest_store s0 r0") apply(force) apply(simp)
+         apply(rename_tac p0)
+         (* this case should be impossible because n0 was not 0, but we got a leaf ; by wf of store; sledgehammer should get this *)
+         apply(simp add: wf_store_def wf_store_page_ref_to_map_def)
+         apply(erule conjE)
+         apply(erule exE)
+         apply(rename_tac m2)
+         apply(simp add: page_ref_to_map_def page_ref_to_kvs_def Let_def)
+         apply(simp add: find_state_to_page_ref_def page_ref_to_frame_def)
+         apply(simp add: ref_to_page_def)
+         apply(simp add: rev_apply_def)
+         apply(force simp add: rresult_to_option_def)  (* sledgehammer should get this *)
+        (* end page_ref_to_tree (ctxt_p2f_t.truncate ctxt1) s0 r0 n0 = none *)
+
+        (* page_ref_to_tree = Some a *)
+        apply(rename_tac t0)
+        apply(case_tac n0)
+         apply(force)
+
+         (* n0 = suc nat *)
+         apply(rename_tac n0')
+         apply(force)
+
+       (* page_ref_to_kvs = Some a *)
+       apply(rename_tac kvs)
+       apply(simp)
+       (* but m0 = none, so can't have kvs = some *)
+       apply(force simp add:rev_apply_def)
+
+      (* m0 = some a *)
+      apply(rename_tac m1)
+      apply(simp)
+      apply(thin_tac "m0 = ?x")
+      apply(simp)
+      apply(simp add: page_ref_to_map_def)
+      apply(simp add: rev_apply_def)
+      apply(elim exE conjE)
+      apply(simp add: page_ref_to_kvs_def rev_apply_def)
+      apply(case_tac n0)
+       (* 0 *)
+       apply(simp)
+       apply(simp add: rev_apply_def)
+       apply(simp add: kvs_to_map_def)
+       apply(drule_tac t=z in sym)
+       apply(simp)
+       apply(thin_tac "z=?x")
+       apply(subgoal_tac "fsl = (| fsl_k = k0, fsl_r = r0 |)") prefer 2 apply(force)
+       apply(simp)
+       apply(simp add:page_ref_to_frame_def)
+       apply(case_tac "ref_to_page s0 r0") apply(force)
+       apply(rename_tac p0)
+       apply(simp)
+       apply(simp add: ref_to_page_def)
+       apply(subgoal_tac "? kvs. lf = (| lf_kvs=kvs |)") prefer 2 apply (metis leaf_frame.cases)  
+       apply(elim exE)
+       apply(simp)
+       apply(thin_tac "lf=?x")
+       apply(thin_tac "fsl=?x")
+       apply(thin_tac "n0=0")
+       apply(clarsimp)
+       apply(force simp add: key_to_v_def rev_apply_def)
+
+       (* suc - should be a contradiction with leaf frame *)
+       apply(rename_tac n0')
+       apply(force)
+  done
 
 end
